Cleaning up code.

Refinement.v
@@ -6,9 +6,9 @@
   - How to handle frame rules? What can change and what cannot?
 *)
 
-Require Import Bool.
-
 Module Refinement.
+
+Require Import Bool.
 
 Record S : Type := mkS {varN : nat; varP : nat; varQ : nat; varR : nat}.
 
@@ -44,19 +44,17 @@ Inductive Refines (pt1 pt2 : PT) : Type :=
     forall (d : pre pt1 ⊂ pre pt2), 
       (forall (s : S) (x : pre pt1 s), post pt2 s (d s x) ⊂ post pt1 s x) -> Refines pt1 pt2.
 
-Notation "PT1 ⊑ PT2" := (Refines PT1 PT2) (at level 90) : type_scope.
+Notation "PT1 ⊏ PT2" := (Refines PT1 PT2) (at level 90, no associativity) : type_scope.
 
 Notation "[ p , q ]" := (Predicate p q) (at level 70) : type_scope.
 
 Ltac refine_simpl := unfold subset, pre, post, extend; simpl; auto.
 
-(*** Guarded command language ***)
-
 (*** Structural laws ***)
 
 Lemma strengthenPost (P : Pow S) (Q1 Q2 : forall s, P s -> Pow S) :
   (forall (s : S) (p : P s), Q1 s p ⊂ Q2 s p) -> 
-  [ P , Q2 ] ⊑ [ P , Q1 ].
+  [ P , Q2 ] ⊏ [ P , Q1 ].
 Proof.
   intros.
   set (d := fun (s : S) (H: P s) => H).
@@ -66,7 +64,7 @@ Proof.
 Qed.
 
 Lemma weakenPre (P1 P2 : Pow S) (Q : forall s, P2 s -> Pow S) (f : P1 ⊂ P2) :
-  [ P1 , (fun s p s' => Q s (f s p) s') ] ⊑ [ P2 , Q ].
+  [ P1 , (fun s p s' => Q s (f s p) s') ] ⊏ [ P2 , Q ].
 Proof.
   intros.
   apply (Refinement ([P1, fun (s : S) (p : P1 s) (s' : S) => Q s (f s p) s']) ([P2, Q]) f).
@@ -76,25 +74,25 @@ Qed.
 
 (*** SKIP **)
 
-Definition Skip : PT := 
+Definition Skip_PT : PT := 
   let skipPre := fun s => True in
   let skipPost := fun s pres s' => s = s' in
   [skipPre , skipPost].
 
 (* Law 4.1 *)
-Lemma refineSkip (pt : PT) : (forall s (pres : pre pt s), post pt s pres s) -> pt ⊑ Skip.
+Lemma refineSkip (pt : PT) : (forall s (pres : pre pt s), post pt s pres s) -> pt ⊏ Skip_PT.
   Proof.
-    intros H; assert (d : pre pt ⊂ pre Skip) by (unfold subset; simpl pre; auto).
-    apply (Refinement pt Skip d).
+    intros H; assert (d : pre pt ⊂ pre Skip_PT) by (unfold subset; simpl pre; auto).
+    apply (Refinement pt Skip_PT d).
     simpl subset; intros s pres s' eq; rewrite <- eq; auto.
   Qed.
 
-Lemma SkipExtendL (U : Pow S) : extend Skip U ⊂ U.
+Lemma SkipExtendL (U : Pow S) : extend Skip_PT U ⊂ U.
   Proof.
     unfold extend; simpl subset; intros s [P1 P2]; apply P2; auto.
   Qed.
 
-Lemma SkipExtendR (U : Pow S) : U ⊂ extend Skip U.
+Lemma SkipExtendR (U : Pow S) : U ⊂ extend Skip_PT U.
   Proof.
     unfold extend, subset; intros s Us; simpl; split; [trivial | intros s' eq; rewrite <- eq; now trivial].
   Qed.
@@ -102,26 +100,26 @@ Lemma SkipExtendR (U : Pow S) : U ⊂ extend Skip U.
 
 (*** ASSIGNMENT ***)
 
-Definition Assign : (S -> S) -> PT := fun f =>
+Definition Assign_PT : (S -> S) -> PT := fun f =>
   let assignPre := fun s => True in
   let assignPost := fun s _ s' => s' = f s in
   [assignPre , assignPost].
 
 (* Law 1.3 *)
-Lemma refineAssign (pt : PT) (f : S -> S) (h : forall (s : S) (pre : pre pt s), post pt s pre (f s)) 
-  : pt ⊑ Assign f.
+Lemma refineAssign (pt : PT) (f : S -> S) (h : forall (s : S) (pre : pre pt s),  post pt s pre (f s)) 
+  : pt ⊏ Assign_PT f.
   Proof.
-    assert (d : pre pt ⊂ pre (Assign f)); refine_simpl.
-    eapply (Refinement pt (Assign f) d).
+    assert (d : pre pt ⊂ pre (Assign_PT f)); refine_simpl.
+    eapply (Refinement pt (Assign_PT f) d).
     simpl; intros s pres s' eq; rewrite eq; auto.
   Qed.
 
-Lemma AssignExtendL (U : Pow S) (f : S -> S) (s : S) : extend (Assign f) U s -> U (f s).
+Lemma AssignExtendL (U : Pow S) (f : S -> S) (s : S) : extend (Assign_PT f) U s -> U (f s).
   Proof.
     unfold extend; intros [H1 H2]; apply H2; reflexivity.
   Qed.
 
-Lemma AssignExtendR  (U : Pow S) (f : S -> S) (s : S) : U (f s) -> extend (Assign f) U s.
+Lemma AssignExtendR  (U : Pow S) (f : S -> S) (s : S) : U (f s) -> extend (Assign_PT f) U s.
   Proof.
     intros Ufs; unfold extend; simpl; split; [ trivial | unfold subset; intros s' eq; rewrite eq; now trivial].
   Qed.
@@ -129,19 +127,19 @@ Lemma AssignExtendR  (U : Pow S) (f : S -> S) (s : S) : U (f s) -> extend (Assig
 
 (*** SEQUENCING **)
 
-Definition Seq (pt1 pt2 : PT) : PT :=
+Definition Seq_PT (pt1 pt2 : PT) : PT :=
   let seqPre := fun s => {pres : pre pt1 s | forall t, post pt1 s pres t -> pre pt2 t} in
   let seqPost : forall s : S, seqPre s -> Pow S := fun (s : S) (pres : seqPre s) (s' : S) => 
     exists t : S, exists q : post pt1 s (proj1_sig pres) t, post pt2 t (proj2_sig pres t q) s'
   in
   [seqPre , seqPost].
 
-Notation "pt1 ;; pt2" := (Seq pt1 pt2) (at level 52, right associativity).
+Notation "pt1 ;; pt2" := (Seq_PT pt1 pt2) (at level 52, right associativity).
 
 (* Law 4.2 *)
 Lemma refineSeq (Pre Mid Post : Pow S) :
   let pt := [ Pre , fun _ _ s' => Post s' ] in
-  pt ⊑ ([Pre , (fun _ _ s' => Mid s') ] ;; [Mid , (fun _ _ s' => Post s') ]).
+  pt ⊏ ([Pre , (fun _ _ s' => Mid s') ] ;; [Mid , (fun _ _ s' => Post s') ]).
   Proof.
     refine_simpl.
     assert (d : pre (Predicate Pre (K Post)) ⊂ pre ([Pre , (K Mid) ] ;; [Mid , (K Post) ])); refine_simpl.
@@ -152,10 +150,10 @@ Lemma refineSeq (Pre Mid Post : Pow S) :
 
 Lemma refineSeqAssign : forall (f: S -> S) (g: S -> S) (h: S -> S),
   (forall (s : S), h s = g (f s)) -> 
-  Assign h ⊑ Assign f ;; Assign g.
+  Assign_PT h ⊏ Assign_PT f ;; Assign_PT g.
 Proof.
   intros.
-  unfold Assign,Seq. simpl.
+  unfold Assign_PT,Seq_PT. simpl.
   assert (d: pre ([fun _ : S => True, fun (s : S) (_ : True) (s' : S) => s' = h s]) ⊂
              pre ([fun s : S => sig (fun _ : True => forall t : S, t = f s -> True),
                    fun (s : S) (_ : sig (fun _ : True => forall t : S, t = f s -> True))
@@ -167,7 +165,7 @@ Proof.
 Qed.
   
 Lemma seqExtendL (pt1 pt2 : PT) (U : Pow S) (s : S) : 
-  extend pt1 (extend pt2 U) s -> extend (Seq pt1 pt2) U s.
+  extend pt1 (extend pt2 U) s -> extend (Seq_PT pt1 pt2) U s.
   Proof.
     refine_simpl.
     intro H; destruct H as [pres posts].
@@ -179,7 +177,7 @@ Lemma seqExtendL (pt1 pt2 : PT) (U : Pow S) (s : S) :
   Qed.
 
 Lemma seqExtendR (pt1 pt2 : PT)  (U : Pow S) (s : S) : 
-  extend (Seq pt1 pt2) U s -> extend pt1 (extend pt2 U) s.
+  extend (Seq_PT pt1 pt2) U s -> extend pt1 (extend pt2 U) s.
   Proof.
    unfold extend, subset; simpl; intro H; destruct H as [[pre1 pre2] post1].
    exists pre1.
@@ -196,7 +194,7 @@ Definition Is_false (b : bool) :=
     | false => True
   end.
 
-Definition If (cond : S -> bool) (Then Else : PT) : PT :=
+Definition If_PT (cond : S -> bool) (Then Else : PT) : PT :=
   let ifPre := fun s => 
     prod (Is_true (cond s) -> pre Then s)
          (Is_false (cond s) -> pre Else s)
@@ -215,17 +213,17 @@ Lemma refineIf (cond : S -> bool) (pt : PT) :
   let elseBranch := [branchPre (fun s => Is_false (cond s)) ,
                      fun s pre s' => post pt s (fst pre) s'  ] in
   
-  pt ⊑ If cond thenBranch elseBranch.
+  pt ⊏ If_PT cond thenBranch elseBranch.
   Proof.
     intros.
     set (d (s : S) (X : pre pt s) := 
       (fun H : Is_true (cond s) => (X,H), fun H : Is_false (cond s) => (X,H))).
-    apply (Refinement pt (If cond thenBranch elseBranch) d).
+    apply (Refinement pt (If_PT cond thenBranch elseBranch) d).
     simpl; intros s pres s'; destruct (cond s); simpl; intros [H1 H2];  auto.
   Qed.
 
 Lemma IfExtendL (cond : S -> bool) (thenPt elsePt : PT) (U : Pow S) (s : S) :
-  extend (If cond thenPt elsePt) U s ->
+  extend (If_PT cond thenPt elsePt) U s ->
     (Is_true (cond s) -> extend thenPt U s) * (Is_false (cond s) -> extend elsePt U s).
   Proof.
     unfold extend; simpl; destruct (cond s); simpl; split; try contradiction;
@@ -238,7 +236,7 @@ Lemma IfExtendL (cond : S -> bool) (thenPt elsePt : PT) (U : Pow S) (s : S) :
 
 Lemma IfExtendR (cond : S -> bool) (thenPt elsePt : PT) (U : Pow S) (s : S) :
     (Is_true (cond s) -> extend thenPt U s) * (Is_false (cond s) -> extend elsePt U s) ->
-    extend (If cond thenPt elsePt) U s.
+    extend (If_PT cond thenPt elsePt) U s.
   Proof.
   unfold extend, subset. simpl; case (cond s); simpl; intros [H1 H2];
   exists (fun t => projT1 (H1 t) , fun f => projT1 (H2 f)).
@@ -246,7 +244,7 @@ Lemma IfExtendR (cond : S -> bool) (thenPt elsePt : PT) (U : Pow S) (s : S) :
     intros; apply (projT2 (H2 I)); destruct H as [_ A]; apply A.
   Qed.
 
-Definition While (inv : Pow S) (cond : S -> bool) (body : PT) : PT :=
+Definition While_PT (inv : Pow S) (cond : S -> bool) (body : PT) : PT :=
   let whilePre := (fun s =>   (* The invariant should hold initially *)
                              inv s /\ 
                               (* If we enter the loop, the precondition of the body should hold *)
@@ -261,11 +259,11 @@ Definition While (inv : Pow S) (cond : S -> bool) (body : PT) : PT :=
 Lemma refineWhile (inv : Pow S) (cond : S -> bool) : 
   let pt := [inv , fun _ _ s' => inv s' ] in
   let body := [fun s => inv s /\ Is_true (cond s), (fun _ _ s => inv s)] in
-  pt ⊑ While inv cond body.
+  pt ⊏ While_PT inv cond body.
   Proof.
     intros; simpl in *.
-    assert (d: pre pt ⊂ pre (While inv cond body)).
-    unfold subset, pt,While; simpl; intros; split; [assumption | ].
+    assert (d: pre pt ⊂ pre (While_PT inv cond body)).
+    unfold subset, pt,While_PT; simpl; intros; split; [assumption | ].
     split.
     intros s' H1. 
     destruct H1; split; assumption.
@@ -281,7 +279,7 @@ Definition WhileSemantics  (inv : Pow S) (cond : S -> bool) (body : PT) (U : Pow
     /\ (forall s, Is_false (cond s) /\ inv s -> U s).
 
 Lemma WhileExtendL (inv : Pow S) (cond : S -> bool) (body : PT) (U : Pow S) (s : S) :
-  extend (While inv cond body) U s -> WhileSemantics inv cond body U s.
+  extend (While_PT inv cond body) U s -> WhileSemantics inv cond body U s.
   Proof.
     unfold extend; simpl; intros [[H1 [H2 H3] H4 ]].
     split; [ assumption | split].
@@ -292,7 +290,7 @@ Lemma WhileExtendL (inv : Pow S) (cond : S -> bool) (body : PT) (U : Pow S) (s :
 
 Lemma WhileExtendR (inv : Pow S) (cond : S -> bool) (body : PT) (U : Pow S) (s : S) :
   WhileSemantics inv cond body U s ->
-    extend (While inv cond body) U s.
+    extend (While_PT inv cond body) U s.
   Proof.
     unfold extend; intros [I [T F]]; simpl in *.
     split; [split; [assumption | ] | ].
@@ -302,8 +300,8 @@ Lemma WhileExtendR (inv : Pow S) (cond : S -> bool) (body : PT) (U : Pow S) (s :
 Qed.
     
     
-Definition refineTrans (pt2 pt1 pt3 : PT) : 
-  pt1 ⊑ pt2 -> pt2 ⊑ pt3 -> pt1 ⊑ pt3.
+Definition refineTransPT (pt2 pt1 pt3 : PT) : 
+  pt1 ⊏ pt2 -> pt2 ⊏ pt3 -> pt1 ⊏ pt3.
     intros [pre12 post12] [pre23 post23].
     set (d (s : S) (pre1s : pre pt1 s) := pre23 s (pre12 s pre1s)).
     refine (Refinement pt1 pt3 d _).
@@ -311,13 +309,13 @@ Definition refineTrans (pt2 pt1 pt3 : PT) :
     apply post12; apply post23; auto.
   Defined.
 
-Definition refineRefl (pt : PT) : pt ⊑ pt.
+Definition refineReflPT (pt : PT) : pt ⊏ pt.
   refine (Refinement pt pt (fun s pres => pres) _).
   intros; unfold subset; auto.
   Defined.
 
-Definition refineSplit (pt1 pt2 pt3 pt4 : PT) :
-  (pt1 ⊑ pt3) -> (pt2 ⊑ pt4) -> (pt1 ;; pt2) ⊑ (pt3 ;; pt4).
+Definition refineSplitPT (pt1 pt2 pt3 pt4 : PT) :
+  (pt1 ⊏ pt3) -> (pt2 ⊏ pt4) -> (pt1 ;; pt2) ⊏ (pt3 ;; pt4).
     intros  [d1 f1] [d2 f2].
     set (d (s : S) (pres : pre (pt1;; pt2) s) :=
           existT (fun pres0 : pre pt3 s => forall t : S, post pt3 s pres0 t -> pre pt4 t)
@@ -332,412 +330,24 @@ Definition refineSplit (pt1 pt2 pt3 pt4 : PT) :
     apply f2; auto.
   Defined.
 
-Definition refineSplitIf (pt1 pt2 pt3 pt4 : PT) (cond : S -> bool) :
-  (pt1 ⊑ pt3) -> (pt2 ⊑ pt4) -> If cond pt1 pt2 ⊑ If cond pt3 pt4.
+Definition refineSplitIfPT (pt1 pt2 pt3 pt4 : PT) (cond : S -> bool) :
+  (pt1 ⊏ pt3) -> (pt2 ⊏ pt4) -> If_PT cond pt1 pt2 ⊏ If_PT cond pt3 pt4.
   intros [d1 f1] [d2 f2].
-  set (d (s : S) (X : pre (If cond pt1 pt2) s)
+  set (d (s : S) (X : pre (If_PT cond pt1 pt2) s)
          := (fun C : Is_true (cond s) => d1 s (fst X C),
              fun C : Is_false (cond s) => d2 s (snd X C)) 
-            : pre (If cond pt3 pt4) s).
+            : pre (If_PT cond pt3 pt4) s).
   apply (Refinement _ _ d).    
   simpl; intros s pres s' [H1 H2].
   split; intros; [apply f1; apply H1 | apply f2; apply H2]; auto.
   Defined.
 
-End Refinement.
-
-Module While.
-
-Require Import EqNat.
-Require Import String.
-Require Import Arith.Bool_nat.
-Require Import Div2.
-Require Import Show.
-Import Refinement.
-
-Definition setN : nat -> S -> S := fun x s =>
-  match s with
-    | mkS _ p q r => mkS x p q r
-  end.
-
-Definition setP : nat -> S -> S := fun x s =>
-  match s with
-    | mkS n _ q r => mkS n x q r
-  end.
-
-Definition setQ : nat -> S -> S := fun x s =>
-  match s with
-    | mkS n p _ r => mkS n p x r
-  end.
-
-Definition setR : nat -> S -> S := fun x s =>
-  match s with
-    | mkS n p q _ => mkS n p q x
-  end.
-
-(* Identifiers *) 
-
-Inductive Identifier : Type :=
-  | N : Identifier
-  | P : Identifier
-  | Q : Identifier
-  | R : Identifier.
-
-Definition setIdent (ident: Identifier) (n : nat) : S -> S :=
-  match ident with
-  | N => setN n
-  | P => setP n
-  | Q => setQ n
-  | R => setR n
-end.
-
-Definition getIdent (ident: Identifier) (s : S) : nat := 
-  match ident , s with
-  | N , mkS n _ _ _ => n
-  | P , mkS _ p _ _ => p
-  | Q , mkS _ _ q _ => q
-  | R , mkS _ _ _ r => r
-end.
-
-(* Expressions *)
-
-Inductive Expr : Type :=
-  | Var    : Identifier -> Expr
-  | EConst : nat -> Expr
-  | Plus   : Expr -> Expr -> Expr
-  | Minus  : Expr -> Expr -> Expr
-  | Mult   : Expr -> Expr -> Expr
-  | Div2   : Expr -> Expr.
-
-Inductive BExpr : Type :=
-  | BConst : bool -> BExpr
-  | And    : BExpr -> BExpr -> BExpr
-  | Or     : BExpr -> BExpr -> BExpr
-  | Not    : BExpr -> BExpr
-  | Eq     : Expr -> Expr -> BExpr
-  | Lt     : Expr -> Expr -> BExpr
-  | Le     : Expr -> Expr -> BExpr
-  | Gt     : Expr -> Expr -> BExpr
-  | Ge     : Expr -> Expr -> BExpr.
-
-Fixpoint evalExpr (e: Expr) (s : S) : nat :=
-  match e with
-  | Var n     => (getIdent n) s
-  | EConst n  => n
-  | Plus x y  => evalExpr x s + evalExpr y s
-  | Minus x y => evalExpr x s - evalExpr y s
-  | Mult x y  => evalExpr x s * evalExpr y s
-  | Div2 x    => div2 (evalExpr x s)
-end.
-
-Fixpoint evalBExpr (b: BExpr) (s: S) : bool :=
-  match b with
-  | BConst b  => b 
-  | And b1 b2 => andb (evalBExpr b1 s) (evalBExpr b2 s) 
-  | Or b1 b2  => orb (evalBExpr b1 s) (evalBExpr b2 s)
-  | Not e     => negb (evalBExpr e s)
-  | Eq e1 e2  => beq_nat (evalExpr e1 s) (evalExpr e2 s)
-  | Lt e1 e2  => proj1_sig (nat_lt_ge_bool (evalExpr e1 s) (evalExpr e2 s))
-  | Le e1 e2  => proj1_sig (nat_le_gt_bool (evalExpr e1 s) (evalExpr e2 s))
-  | Gt e1 e2  => proj1_sig (nat_gt_le_bool (evalExpr e1 s) (evalExpr e2 s))
-  | Ge e1 e2  => proj1_sig (nat_ge_lt_bool (evalExpr e1 s) (evalExpr e2 s))
-end.
-
-(* While Language *)
-
-Inductive WhileL : Type :=
-  | WSkip   : WhileL
-  | WAssign : Identifier -> Expr -> WhileL
-  | WSeq    : WhileL -> WhileL -> WhileL
-  | WIf     : BExpr -> WhileL -> WhileL -> WhileL
-  | WWhile  : Pow S -> BExpr -> WhileL -> WhileL
-  | Spec    : PT -> WhileL.
-
-Fixpoint semantics (w: WhileL) : PT :=
-  match w with
-  | WSkip          => Skip
-  | WAssign id exp => Assign (fun s => (setIdent id (evalExpr exp s)) s)
-  | WSeq st1 st2   => Seq (semantics st1) (semantics st2)
-  | WIf c t e      => If (fun s => (evalBExpr c s)) (semantics t) (semantics e)
-  | WWhile inv c b => While inv (fun s => (evalBExpr c s)) (semantics b)
-  | Spec pt        => pt
-end.
-
-Definition wrefines w1 w2 := (semantics w1) ⊑ (semantics w2).
-
-Notation "P1 ≤ P2" := (wrefines P1 P2) (at level 80) : type_scope.
-  
-
-Fixpoint isExecutable (w: WhileL) : Prop :=
-  match w with 
-  | WSkip          => True
-  | WAssign id exp => True
-  | WSeq st1 st2   => (isExecutable st1) /\ (isExecutable st2)
-  | WIf c t e      => (isExecutable t) /\ (isExecutable e)
-  | WWhile inv c b => isExecutable b
-  | Spec pt        => False
-end.
-
-Open Local Scope string_scope.
-
-Definition identToCode (ident: Identifier) : string :=
-  match ident with
-  | N => "n"
-  | P => "p"
-  | Q => "q"
-  | R => "r"
-  end.
-
-Fixpoint exprToCode (e: Expr) : string :=
-  match e with
-  | Var n     => identToCode n
-  | EConst n  => Show.print_nat n
-  | Plus x y  => exprToCode x ++ " + " ++ exprToCode y
-  | Minus x y => exprToCode x ++ " - " ++ exprToCode y
-  | Mult x y  => exprToCode x ++ " * " ++ exprToCode y
-  | Div2 x    => exprToCode x ++ " / 2"
-  end.
-
-Fixpoint bExprToCode (e: BExpr) : string :=
-  match e with
-  | BConst b  => match b with 
-                 | true  => "true"
-                 | false => "false"
-                 end
-  | And b1 b2 => "(" ++ bExprToCode b1 ++ " && " ++ bExprToCode b2 ++ ")"
-  | Or b1 b2  => "(" ++ bExprToCode b1 ++ " || " ++ bExprToCode b2 ++ ")"
-  | Not e     => "!" ++ bExprToCode e
-  | Eq e1 e2  => "(" ++ exprToCode e1 ++ " == " ++ exprToCode e2  ++ ")"
-  | Lt e1 e2  => "(" ++ exprToCode e1 ++ " < " ++ exprToCode e2  ++ ")"
-  | Le e1 e2  => "(" ++ exprToCode e1 ++ " <= " ++ exprToCode e2  ++ ")"
-  | Gt e1 e2  => "(" ++ exprToCode e1 ++ " > " ++ exprToCode e2  ++ ")"
-  | Ge e1 e2  => "(" ++ exprToCode e1 ++ " >= " ++ exprToCode e2  ++ ")"
-  end.
-
-Fixpoint sp (n: nat) : string := 
-   match n with
-   | 0 => ""
-   | Datatypes.S n' => " " ++ (sp n')
-end.
-
-Lemma isExecSeq1 : forall w1 w2, isExecutable (WSeq w1 w2) -> isExecutable w1.
-Proof. intros; destruct H as [H1 H2]; assumption. Qed.
-
-Lemma isExecSeq2 : forall w1 w2, isExecutable (WSeq w1 w2) -> isExecutable w2.
-Proof. intros; destruct H as [H1 H2]; assumption. Qed.
-
-Lemma isExecThen : forall c t e, isExecutable (WIf c t e) -> isExecutable t.
-Proof. intros; destruct H as [H1 H2]; assumption. Qed.
-
-Lemma isExecElse : forall c t e, isExecutable (WIf c t e) -> isExecutable e.
-Proof. intros; destruct H as [H1 H2]; assumption. Qed.
-
-Lemma isExecBody : forall inv c b, isExecutable (WWhile inv c b) -> isExecutable b.
-Proof. intros; assumption. Qed.
-
-Fixpoint toCode (w: WhileL) (p: isExecutable w) (indent: nat) : string :=
-  match w as w' return (isExecutable w' -> nat -> string) with
-  | WSkip           => fun _ _  => ((sp indent) ++ "skip")
-  | WAssign id exp  => fun _ _ => 
-                       ((sp indent) ++ (identToCode id) ++ " := " ++ (exprToCode exp))
-  | WSeq w1 w2      => fun p' i' => 
-                       (toCode w1 (isExecSeq1 w1 w2 p') i') ++ ";\n" ++ 
-                       (toCode w2 (isExecSeq2 w1 w2 p') i')
-  | WIf c t e       => fun p' i' =>
-                       (sp indent) ++ "if " ++ (bExprToCode c) ++ "\n" ++
-                       (sp indent) ++ "then {\n" ++ 
-                       (toCode t (isExecThen c t e p') (i'+4)) ++ " }\n" ++
-                       (sp indent) ++ "else {\n" ++ 
-                       (toCode e (isExecElse c t e p') (i'+4)) ++ " }"
-  | WWhile inv c b  => fun p' i' =>
-                       (sp indent) ++ "while " ++ (bExprToCode c) ++ "{\n" ++
-                       (sp indent) ++ (toCode b (isExecBody inv c b p') (i'+4)) ++ " }"
-  | Spec pt         => fun p' i' => match p' with 
-                                    end
-  end p indent.
-
-Definition whileExample : WhileL :=
-  WSeq WSkip (WSeq (WIf (BConst true) WSkip WSkip) (WAssign P (Plus (Var R) (Var Q)))).
-
-Lemma whileExec : isExecutable whileExample.
-  Proof. unfold isExecutable; simpl; auto. Qed.
-
-Compute (toCode whileExample whileExec 0).
-
-Ltac w2pt_apply t := unfold "≤",semantics; apply t.
-
-Definition wrefineTrans (w2 w1 w3 : WhileL) : 
-  w1 ≤ w2 -> w2 ≤ w3 -> w1 ≤ w3.
-    w2pt_apply refineTrans.
-  Defined.
-
-Definition wrefineRefl (w : WhileL) :
-  w ≤ w.
-    w2pt_apply refineRefl.
-  Defined.
-
-End While.
-
-
-Module Example.
-
-Require Import Div2.
-Require Import Even.
-Require Import Arith.
-Require Import Arith.Bool_nat.
-Require Import AuxiliaryProofs.
-Import Refinement.
-Import While.
-
-Definition square : nat -> nat := fun n => n * n.
-
-Definition Inv : S -> Prop := fun X => square (varR X) <= varN X < square (varQ X).
-
-Definition SPEC := 
-  ([ (fun _ => True), fun _ _ X => square (varR X) <= varN X < square (1 + varR X)]).
-
-Definition PT1 :=
-  ([ fun _ => True, fun _ _ X => Inv X /\ 1 + varR X = varQ X]).
-
-Ltac refine_post pt1 pt2 := apply (Refinement _ _ (fun s (y : pre pt1 s) => y : pre pt2 s)).
-
-Definition WSPEC := Spec SPEC.
-
-Definition WPT1 := Spec PT1.
-
-Lemma step1 : WSPEC ≤ WPT1.
-  Proof.    
-    unfold WSPEC, WPT1, "≤", semantics. 
-    unfold SPEC, PT1, Inv. refine_post SPEC PT1.
-    intros X tt s [H1 H2]; simpl in *; rewrite H2; apply H1.    
-  Qed.
-
-Definition PT2 := [fun _ => True , K Inv] ;; 
-                  [Inv, fun _ _ X => Inv X /\ 1 + varR X = varQ X].
-
-Definition WPT2 := WSeq (Spec ([fun _ => True , K Inv])) (Spec ([Inv, fun _ _ X => Inv X /\ 1 + varR X = varQ X])).
-
-Lemma step2 : WPT1 ≤ WPT2.
-  Proof.
-    unfold WPT1, WPT2, "≤", semantics. 
-    unfold PT1, PT2, Inv, Seq. simpl.
-    assert (d : forall s, pre PT1 s -> pre PT2 s).
-    intros; exists I; intros; auto.
-    apply (Refinement _ _ d).
-    simpl; intros s Pre s' [t [H1 [H2 H3]]]; split; auto.
-Qed.
-
-Definition PT3a :=
-  Assign (fun s => mkS (varN s) (varP s) (1 + (varN s)) 0).
-
-Definition WPT3aa :=
-  WAssign R (EConst 0).
-
-Definition WPT3ab :=
-  WAssign Q (Plus (EConst 1) (Var N)).
-
-Definition WPT3a := WSeq WPT3aa WPT3ab.
-
-Definition PT3b :=
-  While Inv (fun X => negb (beq_nat (1 + varR X) (varQ X)))
-        ([(fun s => Inv s /\ Is_true (negb (beq_nat (1 + varR s) (varQ s)))),
-          (fun _ _ s' => Inv s')]).
-
-Definition WBody := 
-  Spec ([(fun s => Inv s /\ Is_true (negb (beq_nat (1 + varR s) (varQ s)))),
-          (fun _ _ s' => Inv s')]).  
-
-Definition WPT3b :=
-  let guard := (Not (Eq (Plus (EConst 1) (Var R)) (Var Q))) in
-  WWhile Inv guard WBody.
-
-Lemma step3 : WPT2 ≤ WSeq WPT3a WPT3b.
-Proof.
-  unfold WPT2,WPT3a,WPT3aa,WPT3ab,WPT3b,"≤",semantics.
-  apply refineSplit.
-  simpl.
-  unfold Assign, K, Inv.
-  apply (refineTrans PT3a).
-  (* Part a *)
-    unfold K, Inv, PT3a, square; apply refineAssign.
-    simpl; intros; split; auto with arith.
-  (* refineTrans *)
-  unfold PT3a,Assign.
-  apply refineSeqAssign.
-  intros; destruct s; simpl; reflexivity.
-  (* Part b *)
-     (* FIXME: use refineWhile? *)
-     assert (d: pre ([Inv, fun (s: S) (_: Inv s) (X: S) => Inv X /\ 1 + varR X = varQ X])
-                ⊂ pre (semantics WPT3b)).
-     unfold WPT3b,subset,pre; simpl; intros; split; try assumption.
-     split. 
-     split; inversion H0; assumption.
-     intros; assumption.
-     apply (Refinement _ _ d).
-     intros s Pre s' [Post1 Post2]; split; auto.
-     case_eq (beq_nat (Datatypes.S (varR s')) (varQ s')).
-     intro H; apply (beq_nat_true (Datatypes.S (varR s')) (varQ s') H).
-     change (Is_false (negb (beq_nat (Datatypes.S (varR s')) (varQ s')))) in Post2.
-     intro F; rewrite F in Post2; contradiction.
-Qed.
-
-Definition PT4 := 
-  [fun X => 1 + varR X < varQ X, fun _ _ X => varR X < varP X < varQ X];;
-  [fun X => varR X < varP X < varQ X /\ Inv X, fun _ _ X => Inv X].
-
-Definition WPT4 :=
-  WSeq (Spec ([fun X => 1 + varR X < varQ X /\ Inv X, 
-               fun _ _ X => varR X < varP X < varQ X /\ Inv X]))
-       (Spec ([fun X => varR X < varP X < varQ X /\ Inv X, fun _ _ X => Inv X])).
-
-Axiom lt_n_sq : forall (m n : nat), m < n -> m * m < n * n. 
-
-Axiom lt_sq_n : forall (m n : nat), m * m < n * n -> m < n.
-
-Lemma step4 : WBody ≤ WPT4.
-  unfold WPT3b,WPT4,"≤",semantics; simpl.
-
-  assert (d: pre (semantics WBody) ⊂ pre (semantics WPT4)).
-  unfold subset,pre,semantics,WBody,WPT4.
-  simpl; intros.
-  split. 
-  inversion H as [H1 H2]; inversion H1 as [H3 H4].
-  split. 
-  unfold square in *; destruct s as [N P Q R]; unfold Inv in *; simpl in *.
-  unfold Is_true,negb in H2.
-  remember (if match Q with
-             | 0 => false
-             | Datatypes.S m1 => beq_nat R m1
-             end
-          then false
-          else true) as e.
-  destruct e; induction Q as [|Q HQ]. 
-  unfold square in H4; simpl in H; inversion H4.
-  remember (beq_nat R Q) as beq; destruct beq; inversion Heqe. 
-  symmetry in Heqbeq; apply beq_nat_false in Heqbeq.
-  unfold not in Heqbeq; clear H2; clear Heqe.
-  unfold square in *.
-  apply le_lt_trans with (p:=Datatypes.S Q * Datatypes.S Q) in H3.
-  apply lt_sq_n in H3; unfold "<" in H3; inversion H3. 
-  exfalso; apply Heqbeq; assumption.
-  subst; unfold "<"; apply le_n_S; assumption.
-  assumption.
-  exfalso; assumption.
-  exfalso; assumption.
-  assumption.
-  intros s' [H1 H2]; inversion H as [H3 H4]; split; assumption.
-
-  apply (Refinement _ _ d).
-  intros s PreS; unfold post,subset in *; simpl in *.
-  intros; inversion H as [x [H1 x']]; assumption.
-Qed.
-
-Lemma refineBody : forall (inv : Pow S) (cond : S -> bool) (bodyL bodyR : PT),
-  bodyL ⊑ bodyR ->
-  While inv cond bodyL ⊑ While inv cond bodyR.
+Lemma refineBodyPT : forall (inv : Pow S) (cond : S -> bool) (bodyL bodyR : PT),
+  bodyL ⊏ bodyR ->
+  While_PT inv cond bodyL ⊏ While_PT inv cond bodyR.
 Proof.
   intros inv cond bodyL bodyR [Pre Post].
-  assert (a: pre (While inv cond bodyL) ⊂ pre (While inv cond bodyR)).
+  assert (a: pre (While_PT inv cond bodyL) ⊂ pre (While_PT inv cond bodyR)).
   unfold subset; simpl; intros s [Inv [H1 H2]]; split.
   assumption.
   (* assert (E:  forall s0 : S, Is_true (cond s0) /\ inv s0 -> pre bodyR s0). *)
@@ -751,269 +361,9 @@ Proof.
 
   apply (Refinement _ _ a).
   intros.
-  unfold post,subset,While in *.
+  unfold post,subset,While_PT in *.
   simpl in *.
   intros; assumption.
 Qed.
-  
-Lemma refineBody'' : forall (inv : Pow S) (cond : BExpr) (bodyL bodyR : WhileL),
-  bodyL ≤ bodyR ->
-  WWhile inv cond bodyL ≤ WWhile inv cond bodyR.
-Proof.
-  unfold "≤".
-  intros.
-  assert (d: pre (semantics (WWhile inv cond bodyL)) ⊂
-             pre (semantics (WWhile inv cond bodyR))).
-  unfold subset; simpl; intros s [Inv [H1 H2]]; split.
-  assumption.
-  inversion H as [Pre Post].
-  set (E := fun s0 H => (Pre s0 (H1 _ H))).
-  exists E.
-  intros s0 s' P Q.
-  eapply H2.
-  apply Post.
-  unfold E in Q.
-  exact Q.
 
-  apply (Refinement _ _ d).
-  intros.
-  unfold post,pre,subset in *.
-  simpl in *.
-  intros; assumption.
-Qed.
- 
-Definition PT5a :=
-  Assign (fun s => setP (div2 (varQ s + varR s)) s).
-
-Definition WPT5a :=
-  WAssign P (Div2 (Plus (Var Q) (Var R))).
-
-Definition PT5bThen := 
-  [fun s => (varN s < square (varP s)) /\ (varP s < varQ s) /\ Inv s,
-   fun _ _ s' => Inv s'].
-
-Definition WPT5bThen := Spec PT5bThen.
-
-Definition PT5bElse :=
-  [fun s => (varN s >= square (varP s)) /\ (varR s < varP s) /\ Inv s,
-   fun _ _ s' => Inv s'].
-
-Definition WPT5bElse := Spec PT5bElse.
-
-Definition PT5b :=
-  If (fun s => proj1_sig (nat_lt_ge_bool (varN s) (square (varP s))))
-    PT5bThen PT5bElse.
-
-Definition WPT5b :=
-  WIf (Lt (Var N) (Mult (Var P) (Var P))) WPT5bThen WPT5bElse.
-
-Lemma step5 : WPT4 ≤ WSeq WPT5a WPT5b.
-  unfold "≤",semantics. 
-  simpl.
-  apply refineSplit.
-  apply refineAssign.
-  simpl.
-  intros s H.
-  split.
-  destruct s.
-  simpl in *.
-  split.
-  inversion H as [H1 H2].
-
- (** even-odd approach **)
-  assert (Ha: even varR0 \/ odd varR0).
-  apply even_or_odd. destruct Ha as [R0even|R0odd].
-
-  (* varR0 even *)
-  assert (Ha: even varQ0 \/ odd varQ0). apply even_or_odd. destruct Ha as [Q0even|Q0odd].
-
-  (* varR0 even, varQ0 even *)
-  rewrite <- div2_double at 1. unfold "*". rewrite <- plus_n_O.
-  rewrite even_plus_div2. rewrite even_plus_div2. apply plus_lt_compat_r.
-  apply even_even_lt_div2. split; trivial. apply le_Sn_le in H1. exact H1. trivial. trivial.
-
-  (* varR0 even, varQ0 odd *)
-  rewrite plus_comm. rewrite even_plus_div2. rewrite plus_comm. 
-  rewrite <- div2_double at 1. unfold "*". rewrite <- plus_n_O. rewrite even_plus_div2. 
-  apply plus_lt_compat_r. apply even_odd_lt_div2. split; trivial. trivial. trivial. trivial.
-
-  (* varR0 odd *)
-  assert (Ha: even varQ0 \/ odd varQ0). apply even_or_odd. destruct Ha as [Q0even|Q0odd].
-  
-  (* varR0 odd, varQ0 even *)
-  rewrite <- div2_double at 1. unfold "*". rewrite <- plus_n_O. rewrite odd_odd_plus_div2. 
-  rewrite even_plus_div2. rewrite <- plus_Sn_m. apply plus_lt_compat_r. 
-  apply odd_even_lt_div2. split; trivial. trivial. trivial. split; trivial.
-
-  (* varR0 odd, varQ0 odd *)
-  rewrite <- div2_double at 1. unfold "*". rewrite <- plus_n_O. rewrite odd_odd_plus_div2. 
-  rewrite odd_odd_plus_div2. apply lt_n_S. apply plus_lt_compat_r. apply odd_odd_lt_div2. 
-  split; trivial. apply le_Sn_le in H1. trivial. split; trivial. split; trivial.
-  (** end goal **)
-
-  inversion H as [H1 H2].
-
-  (** even-odd approach **)
-  assert (Ha: even varR0 \/ odd varR0). apply even_or_odd. destruct Ha as [R0even|R0odd].
-  (* varR0 even *)
-  assert (Ha: even varQ0 \/ odd varQ0). apply even_or_odd. destruct Ha as [Q0even|Q0odd].
-  
-  (* varR0 even, varQ0 even *)
-  rewrite <- div2_double. unfold "*". rewrite <- plus_n_O. rewrite even_plus_div2. 
-  rewrite even_plus_div2. rewrite plus_comm. apply plus_lt_compat_r. 
-  apply even_even_lt_div2. split; trivial. apply le_Sn_le in H1. exact H1. trivial. trivial.
-
-  (* varR0 even, varQ0 odd *)
-  rewrite <- div2_double. unfold "*". rewrite <- plus_n_O. rewrite plus_comm. 
-  rewrite even_plus_div2. rewrite odd_odd_plus_div2. rewrite <- plus_Sn_m. 
-  apply plus_lt_compat_r. apply lt_S. apply even_odd_lt_div2. split; trivial. trivial. 
-  split; trivial. trivial.
-
-  (* varR0 odd *)
-  assert (Ha: even varQ0 \/ odd varQ0). apply even_or_odd. destruct Ha as [Q0even|Q0odd].
-  
-  (* varR0 odd, varQ0 even *)
-  rewrite <- div2_double. unfold "*". rewrite <- plus_n_O. rewrite even_plus_div2. 
-  rewrite even_plus_div2. rewrite plus_comm. apply plus_lt_compat_r. apply le_Sn_le. 
-  apply odd_even_lt_div2. split; trivial. trivial. trivial. trivial.
-
-  (* varR0 odd, varQ0 odd *)
-  rewrite <- div2_double. unfold "*". rewrite <- plus_n_O. rewrite odd_odd_plus_div2. 
-  rewrite odd_odd_plus_div2. apply lt_n_S. rewrite plus_comm. apply plus_lt_compat_r. 
-  apply odd_odd_lt_div2. split; trivial. apply le_Sn_le in H1. trivial. split; trivial. 
-  split; trivial.
-  (** end goal **)
-
-  inversion H as [H1 [H2 H3]].
-  unfold Inv in *.
-  split; destruct s as [N P Q R]; simpl in *; assumption.  
-
-  unfold PT5bThen,PT5bElse, Inv.
-  (* FIXME: use refineIf ? *)
-  assert (d: pre ([fun X : S => varR X < varP X < varQ X /\ square (varR X) <= varN X < square (varQ X),
-             fun (s : S) (_ : varR s < varP s < varQ s /\ square (varR s) <= varN s < square (varQ s)) 
-             (X : S) => square (varR X) <= varN X < square (varQ X)])
-             ⊂ pre (semantics WPT5b)).
-  unfold pre,semantics,subset,WPT5b; simpl.
-  intros s [[H1 H2] [H3 H4]].
-  split.
-  intros H5; split. 
-  destruct s as [N P Q R]; simpl in *.
-  unfold Is_true in H5.
-  remember (proj1_sig (nat_lt_ge_bool N (P * P))) as e; destruct e.
-  unfold square in *.
-
-  Focus 5.
-  apply (Refinement _ _ d).
-  simpl.
-  unfold subset.
-  intros.
-  inversion x as [H1 H2].
-  unfold Inv in *.
-  assert (Ha: forall b, or (Is_true b) (Is_false b)).
-  intros. destruct b; simpl in *; auto. 
-  destruct s as [N P Q R].
-  simpl in *.
-  inversion H as [H3 H4].
-  assert (H': or (Is_true (proj1_sig (nat_lt_ge_bool N (P * P))))
-                 (Is_false (proj1_sig (nat_lt_ge_bool N (P * P))))) by (apply Ha).
-  inversion H' as [H5 | H5].
-  apply H3 in H5; assumption.
-  apply H4 in H5; assumption.
-
-  Focus 2. exfalso; assumption.
-  Focus 2. split. assumption. 
-  unfold Inv; split; assumption.
-  Focus 2. split. destruct s as [N P Q R]; simpl in *.
-  Focus 2. split. assumption.
-  unfold Inv; split; assumption.
-
-Admitted.
-
-Lemma step6Then : WPT5bThen ≤ WAssign Q (Var P).
-Proof.
-  unfold WPT5bThen,"≤",semantics.
-  apply refineAssign.
-  simpl.
-  intros s H.
-  unfold Inv in *.
-  destruct H as [H1 [H2 [H3 H4]]].
-  destruct s as [N P Q R].
-  simpl in *.
-  split.
-  assumption.
-  assumption.
-Qed.
-
-Lemma step6Then' : PT5bThen ⊑ Assign (fun s => setQ (varP s) s). 
-  apply refineAssign.
-  simpl.
-  intros s H.
-  destruct H as [H1 H2]; destruct H2 as [H2 H3].
-  destruct s as [N P Q R]. unfold Inv.
-  simpl in *. destruct H3 as [H3 H4]. destruct H3.
-  split. 
-  simpl in *. unfold square in *.
-
-Admitted.
-
-Lemma step6Else : WPT5bElse ≤ WAssign R (Var P).
-Proof.
-  unfold WPT5bElse,"≤",semantics.
-  apply refineAssign.
-  simpl.
-  intros s H.
-  destruct H as [H1 [H2 [H3 H4]]].
-  destruct s. unfold Inv in *.
-  simpl in *.
-  split; auto.
-Qed.
-
-Lemma step6Else' : PT5bElse ⊑ Assign (fun s => setR (varP s) s). 
-  apply refineAssign.
-  simpl.
-  intros s H.
-  destruct H as [H1 H2]; destruct H2 as [H2 H3].
-  destruct s. unfold Inv.
-  simpl in *. destruct H3 as [H3 H4]. simpl in *.
-  split; auto.
-Qed.
-
-Definition prgrm := WSeq WPT3a
-  (WWhile Inv (Not (Eq (Plus (EConst 1) (Var R)) (Var Q)))
-          (WSeq WPT5a (WIf (Lt (Var N) (Mult (Var P) (Var P))) 
-                           (WAssign Q (Var P)) 
-                           (WAssign R (Var P))))).
-
-(* FIXME: Create wrefineSplit and wrefineIf *)
-Theorem result : WSPEC ≤ prgrm.
-Proof.
-  apply (wrefineTrans WPT1); try apply step1.
-  apply (wrefineTrans WPT2); try apply step2.
-  apply (wrefineTrans (WSeq WPT3a WPT3b)); try apply step3.
-(*  apply wrefineSplit. apply wrefineRefl *)
-  assert (Ha: WPT3b ≤ (WWhile Inv (Not (Eq (Plus (EConst 1) (Var R)) (Var Q)))
-          (WSeq WPT5a
-             (WIf (Lt (Var N) (Mult (Var P) (Var P))) 
-                (WAssign Q (Var P)) (WAssign R (Var P)))))).
-
-  apply refineBody''.
-  apply (wrefineTrans WPT4); try apply step4.
-  apply (wrefineTrans (WSeq WPT5a WPT5b)). apply step5.
-(*  apply wrefineSplit. apply wrefineRefl *)
-  assert (Ha: WPT5b ≤ (WIf (Lt (Var N) (Mult (Var P) (Var P))) (WAssign Q (Var P))
-                                                               (WAssign R (Var P)))).
-  unfold WPT5b; apply refineSplitIf.
-  apply step6Then.
-  apply step6Else.
-  apply refineSplit; [apply wrefineRefl | apply Ha].
-  apply refineSplit; [apply wrefineRefl | apply Ha].  
-Qed.
-
-Lemma prgrmProof : isExecutable prgrm.
-Proof.  
-  unfold prgrm,isExecutable; simpl; auto.
-Qed.
-
-Require Import String.
-Compute (toCode prgrm prgrmProof 0).
+End Refinement.
