Example.v
@@ -1,0 +1,376 @@
+Module Example.
+
+Require Import Div2.
+Require Import Even.
+Require Import Arith.
+Require Import Arith.Bool_nat.
+Require Import AuxiliaryProofs.
+
+Load While.
+Import While.
+
+Module Definitions.
+
+Import While.Language.
+Require Import Bool.
+
+Definition square : nat -> nat := fun n => n * n.
+
+Definition Inv : S -> Prop := fun X => square (varR X) <= varN X < square (varQ X).
+
+Definition SPEC := 
+  ([ (fun _ => True), fun _ _ X => square (varR X) <= varN X < square (1 + varR X)]).
+
+Definition WSPEC := Spec SPEC.
+
+Definition PT1 :=
+  ([ fun _ => True, fun _ _ X => Inv X /\ 1 + varR X = varQ X]).
+
+Definition WPT1 := Spec PT1.
+
+Definition PT2 := [fun _ => True , K Inv] ;; 
+                  [Inv, fun _ _ X => Inv X /\ 1 + varR X = varQ X].
+
+Definition WPT2 := (Spec ([fun _ => True , K Inv])) ; (Spec ([Inv, fun _ _ X => Inv X /\ 1 + varR X = varQ X])).
+
+Definition PT3a :=
+  Assign_PT (fun s => mkS (varN s) (varP s) (1 + (varN s)) 0).
+
+Definition WPT3aa :=
+  R ::= (EConst 0).
+
+Definition WPT3ab :=
+  Q ::= (Plus (EConst 1) (Var N)).
+
+Definition WPT3a := WPT3aa ; WPT3ab.
+
+Definition PT3b :=
+  While_PT Inv (fun X => negb (beq_nat (1 + varR X) (varQ X)))
+        ([(fun s => Inv s /\ Is_true (negb (beq_nat (1 + varR s) (varQ s)))),
+          (fun _ _ s' => Inv s')]).
+
+Definition WBody := 
+  Spec ([(fun s => Inv s /\ Is_true (negb (beq_nat (1 + varR s) (varQ s)))),
+          (fun _ _ s' => Inv s')]).  
+
+Definition WPT3b :=
+  let guard := (Not (Eq (Plus (EConst 1) (Var R)) (Var Q))) in
+  While Inv guard WBody.
+
+Definition WPT4 :=
+  (Spec ([fun X => 1 + varR X < varQ X /\ Inv X, 
+          fun _ _ X => varR X < varP X < varQ X /\ Inv X])) ;
+  (Spec ([fun X => varR X < varP X < varQ X /\ Inv X, fun _ _ X => Inv X])).
+
+Definition WPT5a :=
+  P ::= (Div2 (Plus (Var Q) (Var R))).
+
+Definition PT5bThen := 
+  [fun s => (varN s < square (varP s)) /\ (varP s < varQ s) /\ Inv s,
+   fun _ _ s' => Inv s'].
+
+Definition WPT5bThen := 
+  Spec ([fun s => (varN s < square (varP s)) /\ (varP s < varQ s) /\ Inv s,
+         fun _ _ s' => Inv s']).
+
+Definition WPT5bElse := 
+  Spec ([fun s => (varN s >= square (varP s)) /\ (varR s < varP s) /\ Inv s,
+         fun _ _ s' => Inv s']).
+
+Definition WPT5b :=
+  If (Lt (Var N) (Mult (Var P) (Var P))) WPT5bThen WPT5bElse.
+
+End Definitions.
+
+Module Proof.
+
+Import Definitions.
+Import While.CodeGeneration.
+Import Bool.
+
+Ltac refine_post pt1 pt2 := apply (Refinement _ _ (fun s (y : pre pt1 s) => y : pre pt2 s)).
+
+Lemma step1 : WSPEC ⊑ WPT1.
+  Proof.    
+    unfold WSPEC, WPT1, "⊑", semantics. 
+    unfold SPEC, PT1, Inv. refine_post SPEC PT1.
+    intros X tt s [H1 H2]; simpl in *; rewrite H2; apply H1.    
+  Qed.
+
+Lemma step2 : WPT1 ⊑ WPT2.
+  Proof.
+    unfold WPT1, WPT2, "⊑", semantics. 
+    unfold PT1, PT2, Inv, Seq_PT. simpl.
+    assert (d : forall s, pre PT1 s -> pre PT2 s).
+    intros; exists I; intros; auto.
+    apply (Refinement _ _ d).
+    simpl; intros s Pre s' [t [H1 [H2 H3]]]; split; auto.
+Qed.
+
+Lemma step3 : WPT2 ⊑ WPT3a ; WPT3b.
+Proof.
+  unfold WPT2,WPT3a,WPT3aa,WPT3ab,WPT3b,"⊑",semantics.
+  apply refineSplitPT.
+  simpl.
+  unfold Assign_PT, K, Inv.
+  apply (refineTransPT PT3a).
+  (* Part a *)
+    unfold K, Inv, PT3a, square; apply refineAssign.
+    simpl; intros; split; auto with arith.
+  (* refineTrans *)
+  unfold PT3a,Assign_PT.
+  apply refineSeqAssign.
+  intros; destruct s; simpl; reflexivity.
+  (* Part b *)
+     (* FIXME: use refineWhile? *)
+     assert (d: pre ([Inv, fun (s: S) (_: Inv s) (X: S) => Inv X /\ 1 + varR X = varQ X])
+                ⊂ pre (semantics WPT3b)).
+     unfold WPT3b,subset,pre; simpl; intros; split; try assumption.
+     split. 
+     split; inversion H0; assumption.
+     intros; assumption.
+     apply (Refinement _ _ d).
+     intros s Pre s' [Post1 Post2]; split; auto.
+     case_eq (beq_nat (Datatypes.S (varR s')) (varQ s')).
+     intro H; apply (beq_nat_true (Datatypes.S (varR s')) (varQ s') H).
+     change (Is_false (negb (beq_nat (Datatypes.S (varR s')) (varQ s')))) in Post2.
+     intro F; rewrite F in Post2; contradiction.
+Qed.
+
+Axiom lt_n_sq : forall (m n : nat), m < n -> m * m < n * n. 
+Axiom lt_sq_n : forall (m n : nat), m * m < n * n -> m < n.
+
+Lemma step4 : WBody ⊑ WPT4.
+  unfold WPT3b,WPT4,"⊑",semantics; simpl.
+
+  assert (d: pre (semantics WBody) ⊂ pre (semantics WPT4)).
+  unfold subset,pre,semantics,WBody,WPT4.
+  simpl; intros.
+  split. 
+  inversion H as [H1 H2]; inversion H1 as [H3 H4].
+  split. 
+  unfold square in *; destruct s as [N P Q R]; unfold Inv in *; simpl in *.
+  unfold Is_true,negb in H2.
+  remember (if match Q with
+             | 0 => false
+             | Datatypes.S m1 => beq_nat R m1
+             end
+          then false
+          else true) as e.
+  destruct e; induction Q as [|Q HQ]. 
+  unfold square in H4; simpl in H; inversion H4.
+  remember (beq_nat R Q) as beq; destruct beq; inversion Heqe. 
+  symmetry in Heqbeq; apply beq_nat_false in Heqbeq.
+  unfold not in Heqbeq; clear H2; clear Heqe.
+  unfold square in *.
+  apply le_lt_trans with (p:=Datatypes.S Q * Datatypes.S Q) in H3.
+  apply lt_sq_n in H3; unfold "<" in H3; inversion H3. 
+  exfalso; apply Heqbeq; assumption.
+  subst; unfold "<"; apply le_n_S; assumption.
+  assumption.
+  exfalso; assumption.
+  exfalso; assumption.
+  assumption.
+  intros s' [H1 H2]; inversion H as [H3 H4]; split; assumption.
+
+  apply (Refinement _ _ d).
+  intros s PreS; unfold post,subset in *; simpl in *.
+  intros; inversion H as [x [H1 x']]; assumption.
+Qed.
+
+
+Lemma step5 : WPT4 ⊑ WPT5a ; WPT5b.
+  unfold "⊑",semantics. 
+  simpl.
+  apply refineSplitPT.
+  apply refineAssign.
+  simpl.
+  intros s H.
+  split.
+  destruct s.
+  simpl in *.
+  split.
+  inversion H as [H1 H2].
+
+ (** even-odd approach **)
+  assert (Ha: even varR0 \/ odd varR0).
+  apply even_or_odd. destruct Ha as [R0even|R0odd].
+
+  (* varR0 even *)
+  assert (Ha: even varQ0 \/ odd varQ0). apply even_or_odd. destruct Ha as [Q0even|Q0odd].
+
+  (* varR0 even, varQ0 even *)
+  rewrite <- div2_double at 1. unfold "*". rewrite <- plus_n_O.
+  rewrite even_plus_div2. rewrite even_plus_div2. apply plus_lt_compat_r.
+  apply even_even_lt_div2. split; trivial. apply le_Sn_le in H1. exact H1. trivial. trivial.
+
+  (* varR0 even, varQ0 odd *)
+  rewrite plus_comm. rewrite even_plus_div2. rewrite plus_comm. 
+  rewrite <- div2_double at 1. unfold "*". rewrite <- plus_n_O. rewrite even_plus_div2. 
+  apply plus_lt_compat_r. apply even_odd_lt_div2. split; trivial. trivial. trivial. trivial.
+
+  (* varR0 odd *)
+  assert (Ha: even varQ0 \/ odd varQ0). apply even_or_odd. destruct Ha as [Q0even|Q0odd].
+  
+  (* varR0 odd, varQ0 even *)
+  rewrite <- div2_double at 1. unfold "*". rewrite <- plus_n_O. rewrite odd_odd_plus_div2. 
+  rewrite even_plus_div2. rewrite <- plus_Sn_m. apply plus_lt_compat_r. 
+  apply odd_even_lt_div2. split; trivial. trivial. trivial. split; trivial.
+
+  (* varR0 odd, varQ0 odd *)
+  rewrite <- div2_double at 1. unfold "*". rewrite <- plus_n_O. rewrite odd_odd_plus_div2. 
+  rewrite odd_odd_plus_div2. apply lt_n_S. apply plus_lt_compat_r. apply odd_odd_lt_div2. 
+  split; trivial. apply le_Sn_le in H1. trivial. split; trivial. split; trivial.
+  (** end goal **)
+
+  inversion H as [H1 H2].
+
+  (** even-odd approach **)
+  assert (Ha: even varR0 \/ odd varR0). apply even_or_odd. destruct Ha as [R0even|R0odd].
+  (* varR0 even *)
+  assert (Ha: even varQ0 \/ odd varQ0). apply even_or_odd. destruct Ha as [Q0even|Q0odd].
+  
+  (* varR0 even, varQ0 even *)
+  rewrite <- div2_double. unfold "*". rewrite <- plus_n_O. rewrite even_plus_div2. 
+  rewrite even_plus_div2. rewrite plus_comm. apply plus_lt_compat_r. 
+  apply even_even_lt_div2. split; trivial. apply le_Sn_le in H1. exact H1. trivial. trivial.
+
+  (* varR0 even, varQ0 odd *)
+  rewrite <- div2_double. unfold "*". rewrite <- plus_n_O. rewrite plus_comm. 
+  rewrite even_plus_div2. rewrite odd_odd_plus_div2. rewrite <- plus_Sn_m. 
+  apply plus_lt_compat_r. apply lt_S. apply even_odd_lt_div2. split; trivial. trivial. 
+  split; trivial. trivial.
+
+  (* varR0 odd *)
+  assert (Ha: even varQ0 \/ odd varQ0). apply even_or_odd. destruct Ha as [Q0even|Q0odd].
+  
+  (* varR0 odd, varQ0 even *)
+  rewrite <- div2_double. unfold "*". rewrite <- plus_n_O. rewrite even_plus_div2. 
+  rewrite even_plus_div2. rewrite plus_comm. apply plus_lt_compat_r. apply le_Sn_le. 
+  apply odd_even_lt_div2. split; trivial. trivial. trivial. trivial.
+
+  (* varR0 odd, varQ0 odd *)
+  rewrite <- div2_double. unfold "*". rewrite <- plus_n_O. rewrite odd_odd_plus_div2. 
+  rewrite odd_odd_plus_div2. apply lt_n_S. rewrite plus_comm. apply plus_lt_compat_r. 
+  apply odd_odd_lt_div2. split; trivial. apply le_Sn_le in H1. trivial. split; trivial. 
+  split; trivial.
+  (** end goal **)
+
+  inversion H as [H1 [H2 H3]].
+  unfold Inv in *.
+  split; destruct s as [N P Q R]; simpl in *; assumption.  
+
+  unfold Inv.
+  (* FIXME: use refineIf ? *)
+  assert (d: pre ([fun X : S => varR X < varP X < varQ X /\ square (varR X) <= varN X < square (varQ X),
+             fun (s : S) (_ : varR s < varP s < varQ s /\ square (varR s) <= varN s < square (varQ s)) 
+             (X : S) => square (varR X) <= varN X < square (varQ X)])
+             ⊂ pre (semantics WPT5b)).
+  unfold pre,semantics,subset,WPT5b; simpl.
+  intros s [[H1 H2] [H3 H4]].
+  destruct s as [N P Q R]; simpl in *.
+  split.
+  intros H5; split. 
+  unfold Is_true in H5.  
+  remember (Compare_dec.leb N (P * P) && negb (beq_nat N (P * P))) as e; destruct e.
+  symmetry in Heqe; apply andb_true_iff in Heqe.
+  inversion Heqe as [H6 H7].
+  apply leb_iff in H6.
+  unfold square,"<"; unfold negb in H7.
+  remember (beq_nat N (P * P)) as e; destruct e.
+  inversion H7.
+  symmetry in Heqe0.
+  apply beq_nat_false in Heqe0.
+  inversion H6.
+  contradiction.
+  apply le_n_S; assumption.
+  exfalso; assumption.
+  split; [assumption | unfold Inv; split; assumption].
+  intros; split.
+  unfold Is_false in H.
+  remember (Compare_dec.leb N (P * P) && negb (beq_nat N (P * P))) as e; destruct e.
+  exfalso; assumption.
+  symmetry in Heqe; apply andb_false_iff in Heqe.
+  inversion Heqe as [H5 | H5].
+  apply leb_complete_conv in H5.
+  unfold square,ge,lt in *; apply le_Sn_le in H5; assumption.
+  unfold negb in H5; remember (beq_nat N (P * P)) as e; destruct e.
+  symmetry in Heqe0; apply beq_nat_true in Heqe0.
+  unfold ge,square in *; symmetry in Heqe0.
+  rewrite Heqe0; apply le_n.
+  inversion H5.
+  split; [assumption | unfold Inv; split; assumption].
+
+  apply (Refinement _ _ d).
+  simpl; unfold subset; intros.
+  inversion x as [H1 H2].
+  unfold Inv in *.
+  assert (Ha: forall b, or (Is_true b) (Is_false b)) by 
+         (intros; destruct b; simpl in *; auto). 
+  destruct s as [N P Q R]; simpl in *.
+  inversion H as [H3 H4]. 
+  assert (H': or (Is_true (Compare_dec.leb N (P * P) && negb (beq_nat N (P * P))))
+                 (Is_false (Compare_dec.leb N (P * P) && negb (beq_nat N (P * P)))))
+         by (apply Ha).
+  inversion H' as [H5 | H5].
+  apply H3 in H5; assumption.
+  apply H4 in H5; assumption.
+Qed.
+
+Lemma step6Then : WPT5bThen ⊑ Q ::= (Var P).
+Proof.
+  unfold WPT5bThen,"⊑",semantics.
+  apply refineAssign.
+  simpl.
+  intros s H.
+  unfold Inv in *.
+  destruct H as [H1 [H2 [H3 H4]]].
+  destruct s as [N P Q R].
+  simpl in *.
+  split.
+  assumption.
+  assumption.
+Qed.
+
+Lemma step6Else : WPT5bElse ⊑ R ::= (Var P).
+Proof.
+  unfold WPT5bElse,"⊑",semantics.
+  apply refineAssign.
+  simpl.
+  intros s H.
+  destruct H as [H1 [H2 [H3 H4]]].
+  destruct s. unfold Inv in *.
+  simpl in *.
+  split; auto.
+Qed.
+
+Definition prgrm := WPT3a ;
+  (While Inv (Not (Eq (Plus (EConst 1) (Var R)) (Var Q)))
+         (WPT5a ; (If (Lt (Var N) (Mult (Var P) (Var P))) 
+                      (Q ::= (Var P)) 
+                      (R ::= (Var P))))).
+
+Theorem result : WSPEC ⊑ prgrm.
+Proof.
+  apply (refineTrans WPT1); try apply step1.
+  apply (refineTrans WPT2); try apply step2.
+  apply (refineTrans (WPT3a ; WPT3b)); try apply step3.
+  apply refineSplit; try apply refineRefl.
+  unfold WPT3b; apply refineBody.
+  apply (refineTrans WPT4); try apply step4.
+  apply (refineTrans (WPT5a ; WPT5b)); try apply step5.
+  apply refineSplit; try apply refineRefl.
+  unfold WPT5b; apply refineSplitIf; [apply step6Then | apply step6Else]. 
+Qed.
+
+Lemma prgrmProof : isExecutable prgrm.
+Proof.  
+  unfold prgrm,isExecutable; simpl; auto.
+Qed.
+
+Require Import String.
+Compute (toCode prgrm prgrmProof 0).
+
+End Proof.
+
+End Example.
