While.v
@@ -1,0 +1,291 @@
+Module While.
+
+Require Import EqNat.
+Require Import String.
+Require Import Arith.Bool_nat.
+Require Import Div2.
+Require Import Show.
+
+Load Refinement.
+Export Refinement.
+
+Module Language.
+
+Definition setN : nat -> S -> S := fun x s =>
+  match s with
+    | mkS _ p q r => mkS x p q r
+  end.
+
+Definition setP : nat -> S -> S := fun x s =>
+  match s with
+    | mkS n _ q r => mkS n x q r
+  end.
+
+Definition setQ : nat -> S -> S := fun x s =>
+  match s with
+    | mkS n p _ r => mkS n p x r
+  end.
+
+Definition setR : nat -> S -> S := fun x s =>
+  match s with
+    | mkS n p q _ => mkS n p q x
+  end.
+
+(* Identifiers *) 
+
+Inductive Identifier : Type :=
+  | N : Identifier
+  | P : Identifier
+  | Q : Identifier
+  | R : Identifier.
+
+(* Expressions *)
+
+Inductive Expr : Type :=
+  | Var    : Identifier -> Expr
+  | EConst : nat -> Expr
+  | Plus   : Expr -> Expr -> Expr
+  | Minus  : Expr -> Expr -> Expr
+  | Mult   : Expr -> Expr -> Expr
+  | Div2   : Expr -> Expr.
+
+Inductive BExpr : Type :=
+  | BConst : bool -> BExpr
+  | And    : BExpr -> BExpr -> BExpr
+  | Or     : BExpr -> BExpr -> BExpr
+  | Not    : BExpr -> BExpr
+  | Eq     : Expr -> Expr -> BExpr
+  | Lt     : Expr -> Expr -> BExpr
+  | Le     : Expr -> Expr -> BExpr
+  | Gt     : Expr -> Expr -> BExpr
+  | Ge     : Expr -> Expr -> BExpr.
+
+(* While Language *)
+
+Inductive WhileL : Type :=
+  | Skip   : WhileL
+  | Assign : Identifier -> Expr -> WhileL
+  | Seq    : WhileL -> WhileL -> WhileL
+  | If     : BExpr -> WhileL -> WhileL -> WhileL
+  | While  : Pow S -> BExpr -> WhileL -> WhileL
+  | Spec   : PT -> WhileL.
+
+Notation "w1 ; w2" := (Seq w1 w2) (at level 52, right associativity).
+Notation "id ::= exp" := (Assign id exp) (at level 52).
+
+End Language.
+
+Module Semantics.
+
+Export Language.
+
+Definition setIdent (ident: Identifier) (n : nat) : S -> S :=
+  match ident with
+  | N => setN n
+  | P => setP n
+  | Q => setQ n
+  | R => setR n
+end.
+
+Definition getIdent (ident: Identifier) (s : S) : nat := 
+  match ident , s with
+  | N , mkS n _ _ _ => n
+  | P , mkS _ p _ _ => p
+  | Q , mkS _ _ q _ => q
+  | R , mkS _ _ _ r => r
+end.
+
+Fixpoint evalExpr (e: Expr) (s : S) : nat :=
+  match e with
+  | Var n     => (getIdent n) s
+  | EConst n  => n
+  | Plus x y  => evalExpr x s + evalExpr y s
+  | Minus x y => evalExpr x s - evalExpr y s
+  | Mult x y  => evalExpr x s * evalExpr y s
+  | Div2 x    => div2 (evalExpr x s)
+end.
+
+Fixpoint evalBExpr (b: BExpr) (s: S) : bool :=
+  match b with
+  | BConst b  => b 
+  | And b1 b2 => andb (evalBExpr b1 s) (evalBExpr b2 s) 
+  | Or b1 b2  => orb (evalBExpr b1 s) (evalBExpr b2 s)
+  | Not e     => negb (evalBExpr e s)
+  | Eq e1 e2  => beq_nat (evalExpr e1 s) (evalExpr e2 s)
+  | Lt e1 e2  => andb (leb (evalExpr e1 s) (evalExpr e2 s)) 
+                      (negb (beq_nat (evalExpr e1 s) (evalExpr e2 s)))
+  | Le e1 e2  => leb (evalExpr e1 s) (evalExpr e2 s)
+  | Gt e1 e2  => negb (leb (evalExpr e1 s) (evalExpr e2 s))
+  | Ge e1 e2  => negb (andb (leb (evalExpr e1 s) (evalExpr e2 s)) 
+                      (negb (beq_nat (evalExpr e1 s) (evalExpr e2 s))))
+(*
+  | Lt e1 e2  => proj1_sig (nat_lt_ge_bool (evalExpr e1 s) (evalExpr e2 s))
+  | Le e1 e2  => proj1_sig (nat_le_gt_bool (evalExpr e1 s) (evalExpr e2 s))
+  | Gt e1 e2  => proj1_sig (nat_gt_le_bool (evalExpr e1 s) (evalExpr e2 s))
+  | Ge e1 e2  => proj1_sig (nat_ge_lt_bool (evalExpr e1 s) (evalExpr e2 s))
+*)
+end.
+
+Fixpoint semantics (w: WhileL) : PT :=
+  match w with
+  | Skip          => Skip_PT
+  | Assign id exp => Assign_PT (fun s => (setIdent id (evalExpr exp s)) s)
+  | Seq st1 st2   => Seq_PT (semantics st1) (semantics st2)
+  | If c t e      => If_PT (fun s => (evalBExpr c s)) (semantics t) (semantics e)
+  | While inv c b => While_PT inv (fun s => (evalBExpr c s)) (semantics b)
+  | Spec pt       => pt
+end.
+
+Definition wrefines w1 w2 := (semantics w1) ⊏ (semantics w2).
+
+Notation "P1 ⊑ P2" := (wrefines P1 P2) (at level 90, no associativity) : type_scope.
+
+Definition refineTrans (w2 w1 w3 : WhileL) : 
+  w1 ⊑ w2 -> w2 ⊑ w3 -> w1 ⊑ w3.
+    unfold "⊑",semantics; apply refineTransPT.
+  Defined.
+
+Definition refineRefl (w : WhileL) :
+  w ⊑ w.
+    unfold "⊑",semantics; apply refineReflPT.
+  Defined.
+
+Definition refineSplit (w1 w2 w3 w4 : WhileL) :
+  (w1 ⊑ w3) -> (w2 ⊑ w4) -> (w1 ; w2) ⊑ (w3 ; w4).
+    unfold "⊑",semantics; apply refineSplitPT.
+  Defined.
+
+Definition refineSplitIf (w1 w2 w3 w4 : WhileL) (cond : BExpr) :
+  (w1 ⊑ w3) -> (w2 ⊑ w4) -> If cond w1 w2 ⊑ If cond w3 w4.
+    unfold "⊑",semantics; apply refineSplitIfPT.
+  Defined.
+
+Definition refineBody : forall (inv : Pow S) (cond : BExpr) (bodyL bodyR : WhileL),
+  bodyL ⊑ bodyR ->
+  While inv cond bodyL ⊑ While inv cond bodyR.
+Proof.
+  unfold "⊑",semantics.
+  intros.
+  assert (d: pre (semantics (While inv cond bodyL)) ⊂
+             pre (semantics (While inv cond bodyR))).
+  unfold subset; simpl; intros s [Inv [H1 H2]]; split.
+  assumption.
+  inversion H as [Pre Post].
+  set (E := fun s0 H => (Pre s0 (H1 _ H))).
+  exists E.
+  intros s0 s' P Q.
+  eapply H2.
+  apply Post.
+  unfold E in Q.
+  exact Q.
+
+  apply (Refinement _ _ d).
+  intros.
+  unfold post,pre,subset in *.
+  simpl in *.
+  intros; assumption.
+Defined.
+
+End Semantics.
+
+Module CodeGeneration.
+
+Export Semantics.
+
+Fixpoint isExecutable (w: WhileL) : Prop :=
+  match w with 
+  | Skip          => True
+  | Assign id exp => True
+  | Seq st1 st2   => (isExecutable st1) /\ (isExecutable st2)
+  | If c t e      => (isExecutable t) /\ (isExecutable e)
+  | While inv c b => isExecutable b
+  | Spec pt       => False
+end.
+
+Open Local Scope string_scope.
+
+Definition identToCode (ident: Identifier) : string :=
+  match ident with
+  | N => "n"
+  | P => "p"
+  | Q => "q"
+  | R => "r"
+  end.
+
+Fixpoint exprToCode (e: Expr) : string :=
+  match e with
+  | Var n     => identToCode n
+  | EConst n  => Show.print_nat n
+  | Plus x y  => exprToCode x ++ " + " ++ exprToCode y
+  | Minus x y => exprToCode x ++ " - " ++ exprToCode y
+  | Mult x y  => exprToCode x ++ " * " ++ exprToCode y
+  | Div2 x    => exprToCode x ++ " / 2"
+  end.
+
+Fixpoint bExprToCode (e: BExpr) : string :=
+  match e with
+  | BConst b  => match b with 
+                 | true  => "true"
+                 | false => "false"
+                 end
+  | And b1 b2 => "(" ++ bExprToCode b1 ++ " && " ++ bExprToCode b2 ++ ")"
+  | Or b1 b2  => "(" ++ bExprToCode b1 ++ " || " ++ bExprToCode b2 ++ ")"
+  | Not e     => "!" ++ bExprToCode e
+  | Eq e1 e2  => "(" ++ exprToCode e1 ++ " == " ++ exprToCode e2  ++ ")"
+  | Lt e1 e2  => "(" ++ exprToCode e1 ++ " < " ++ exprToCode e2  ++ ")"
+  | Le e1 e2  => "(" ++ exprToCode e1 ++ " <= " ++ exprToCode e2  ++ ")"
+  | Gt e1 e2  => "(" ++ exprToCode e1 ++ " > " ++ exprToCode e2  ++ ")"
+  | Ge e1 e2  => "(" ++ exprToCode e1 ++ " >= " ++ exprToCode e2  ++ ")"
+  end.
+
+Fixpoint sp (n: nat) : string := 
+   match n with
+   | 0 => ""
+   | Datatypes.S n' => " " ++ (sp n')
+end.
+
+Lemma isExecSeq1 : forall w1 w2, isExecutable (Seq w1 w2) -> isExecutable w1.
+Proof. intros; destruct H as [H1 H2]; assumption. Qed.
+
+Lemma isExecSeq2 : forall w1 w2, isExecutable (Seq w1 w2) -> isExecutable w2.
+Proof. intros; destruct H as [H1 H2]; assumption. Qed.
+
+Lemma isExecThen : forall c t e, isExecutable (If c t e) -> isExecutable t.
+Proof. intros; destruct H as [H1 H2]; assumption. Qed.
+
+Lemma isExecElse : forall c t e, isExecutable (If c t e) -> isExecutable e.
+Proof. intros; destruct H as [H1 H2]; assumption. Qed.
+
+Lemma isExecBody : forall inv c b, isExecutable (While inv c b) -> isExecutable b.
+Proof. intros; assumption. Qed.
+
+Fixpoint toCode (w: WhileL) (p: isExecutable w) (indent: nat) : string :=
+  match w as w' return (isExecutable w' -> nat -> string) with
+  | Skip           => fun _ _  => ((sp indent) ++ "skip")
+  | Assign id exp  => fun _ _ => 
+                      ((sp indent) ++ (identToCode id) ++ " := " ++ (exprToCode exp))
+  | Seq w1 w2      => fun p' i' => 
+                      (toCode w1 (isExecSeq1 w1 w2 p') i') ++ ";\n" ++ 
+                      (toCode w2 (isExecSeq2 w1 w2 p') i')
+  | If c t e       => fun p' i' =>
+                      (sp indent) ++ "if " ++ (bExprToCode c) ++ "\n" ++
+                      (sp indent) ++ "then \n" ++ 
+                      (sp indent) ++ "{\n" ++ 
+                      (toCode t (isExecThen c t e p') (i'+4)) ++ "\n" ++
+                      (sp indent) ++ "}\n" ++
+                      (sp indent) ++ "else \n" ++ 
+                      (sp indent) ++ "{\n" ++ 
+                      (toCode e (isExecElse c t e p') (i'+4)) ++ "\n" ++
+                      (sp indent) ++ "}"
+  | While inv c b  => fun p' i' =>
+                      (sp indent) ++ "while " ++ (bExprToCode c) ++ "\n" ++
+                      (sp indent) ++ "{\n" ++
+                      (sp indent) ++ (toCode b (isExecBody inv c b p') (i'+4)) ++ "\n" ++
+                      (sp indent) ++ "}"
+  | Spec pt         => fun p' i' => match p' with 
+                                    end
+  end p indent.
+
+End CodeGeneration.
+
+End While.
