Makefile
@@ -1,0 +1,21 @@
+default: coq
+
+coq: show refinement while auxproofs example 
+
+show: 
+	coqc Show.v
+
+refinement:
+	coqc Refinement.v
+
+while: show refinement
+	coqc While.v
+
+auxproofs: 
+	coqc AuxiliaryProofs.v
+
+example: show refinement while auxproofs
+	coqc Example.v
+
+clean:
+	rm -f *.vo *.glob 
